PFPL/ch16.v
@@ -1,0 +1,337 @@
+(* Recursive types *)
+
+Require Import Env.
+Require Import TransitiveClosure.
+
+Inductive Ty :=
+        | t_arr  : Ty -> Ty -> Ty
+        | t_unit : Ty
+        | t_fix  : Ty -> Ty
+        | t_var  : Var -> Ty.
+
+Inductive Exp :=
+        | var    : Var -> Exp
+        | lambda : Ty  -> Exp -> Exp
+        | app    : Exp -> Exp -> Exp
+        | fixx   : Ty  -> Exp -> Exp
+        
+        | fold   : Ty  -> Exp -> Exp
+        | unfold : Exp -> Exp
+        
+        | unitt  : Exp.
+
+
+Definition TTEnv := Env unit.
+Definition TEnv := Env Ty.
+
+
+Fixpoint raiseT (e : Ty) (a b : nat) :=
+ match e with
+ | t_var v     => t_var  (raise' a b v)
+ | t_arr  p q  => t_arr  (raiseT p a b) (raiseT p a b)
+ | t_unit      => t_unit
+ | t_fix  x    => t_fix  (raiseT x a (S b))
+ end.
+
+Fixpoint subT' (e e' : Ty) (v : Var) :=
+ match e with
+ | t_var v'     => subst' v v' t_var e'
+ | t_fix t      => t_fix (subT' t (raiseT e' 1 0) (S v))
+
+ | t_arr  p q  => t_arr  (subT' p e' v) (subT' p e' v)
+ | t_unit      => t_unit
+ end.
+
+Definition subT e e' := subT' e e' 0.
+
+
+Inductive TyWf (env:TTEnv) : Ty -> Prop :=
+ | twf_env v : InEnv v tt env -> TyWf env (t_var v)
+ | twf_arr t1 t2
+   : TyWf env t1
+  -> TyWf env t2
+  -> TyWf env (t_arr t1 t2)
+ | twf_fix t
+   : TyWf (tt :: env) t 
+  -> TyWf        env  (t_fix t)
+
+ | twf_unit : TyWf env t_unit.
+
+(* Is TyWf necessary?
+   Is there a way to make the TyWf[]t requirements neater or less repetitive? *)
+Inductive TYPE (env : TEnv) : Exp -> Ty -> Prop :=
+ | ty_env (v : Var) (t : Ty)
+   : InEnv v t env
+  -> TyWf [] t
+  -> TYPE env (var v) t
+
+ | ty_lam b t1 t2
+   : TYPE (t1 :: env) b t2
+  -> TyWf [] (t_arr t1 t2)
+  -> TYPE env (lambda t1 b) (t_arr t1 t2)
+
+ | ty_app e1 e2 t1 t2
+   : TYPE env e1 (t_arr t1 t2)
+  -> TYPE env e2 t1
+  -> TyWf [] t2
+  -> TYPE env (app e1 e2) t2
+
+ | ty_fixx t e
+   : TYPE (t :: env) e t
+  -> TyWf [] t
+  -> TYPE env (fixx t e) t
+
+
+ | ty_fold t e
+   : TYPE env e          (subT t (t_fix t))
+  -> TyWf [] (t_fix t)
+  -> TYPE env (fold t e) (t_fix t)
+
+ | ty_unfold t e
+   : TYPE env e          (t_fix t)
+  -> TyWf [] (subT t (t_fix t))
+  -> TYPE env (unfold e) (subT t (t_fix t)).
+
+
+Lemma unicity
+	(env: TEnv) (e : Exp) (t1 t2 : Ty)
+	(Ht1 : TYPE env e t1)
+	(Ht2 : TYPE env e t2)
+	: t1 = t2.
+Proof.
+  revert t2 Ht2.
+  induction Ht1; intros; inversion Ht2; subst; try congruence.
+  
+  apply IHHt1 in H2. congruence.
+
+  apply IHHt1_1 in H2. congruence.
+
+  apply IHHt1 in H1. congruence.
+Qed.
+
+
+Fixpoint raise (e : Exp) (a b : nat) :=
+ match e with
+ | var v       => var (raise' a b v)
+ | lambda t x  => lambda t (raise x a (S b))
+ | app f x     => app (raise f a b) (raise x a b)
+ | fixx t x    => fixx t (raise x a (S b))
+
+ | fold t e    => fold t (raise e a b)
+ | unfold e    => unfold (raise e a b)
+
+ | unitt       => unitt
+ end.
+
+Lemma raise_0_id (e : Exp) (n : nat) :
+	raise e 0 n = e.
+Proof.
+ revert n.
+ induction e; intros; simpl; try (rewrite IHe1, IHe2); try rewrite IHe; try rewrite IHe3; try reflexivity.
+ unfold raise, raise'.
+ destruct (ge_dec v n); auto.
+Qed.
+
+Lemma raise_S (e : Exp) (a b : nat) :
+	raise e (S a) b = raise (raise e a b) 1 b.
+Proof.
+ revert a b.
+ induction e; intros; simpl; try (rewrite IHe1, IHe2); try rewrite IHe; try rewrite IHe3; try reflexivity.
+ unfold raise, raise'.
+ destruct (ge_dec v b); auto.
+ destruct (ge_dec (a+v) b); auto.
+  omega.
+ destruct (ge_dec v b); auto.
+  omega. 
+Qed.
+
+
+
+Fixpoint subst (e e' : Exp) (v : Var) :=
+ match e with
+ | var v'       => subst' v v' var e'
+ | lambda t x   => lambda t (subst x (raise e' 1 0) (S v))
+ | app    f x   => app (subst f e' v) (subst x e' v)
+ | fixx   t x   => fixx t (subst x (raise e' 1 0) (S v))
+
+ | fold t e    => fold t (subst e e' v)
+ | unfold e    => unfold (subst e e' v)
+
+ | unitt       => unitt
+ end.
+
+
+
+Lemma weakening_insert
+        (env : TEnv) (e : Exp) (te tvi : Ty) (vi : Var) :
+        TYPE env e te ->
+        TYPE (insert env vi tvi) (raise e 1 vi) te.
+ intros Hte.
+ revert vi tvi.
+ induction Hte; intros; try solve [constructor; auto]; simpl.
+
+ apply ty_env.
+  unfold raise'.
+   destruct (ge_dec v vi).
+   apply get_insert_ge; assumption.
+   apply get_insert_lt; try assumption; omega.
+  assumption.
+
+ apply ty_lam.
+  rewrite <- uninsert.
+  apply IHHte. assumption.
+
+ eapply ty_app; eauto.
+
+ eapply ty_fixx.
+  rewrite <- uninsert; auto.
+  assumption.
+Qed.
+
+Lemma weakening_cons
+	(env : TEnv) (e : Exp) (te : Ty) tv : 
+	TYPE env e te ->
+	TYPE (tv :: env) (raise e 1 0) te.
+Proof.
+ rewrite <- insert_0.
+ apply weakening_insert.
+Qed.
+
+
+
+
+Lemma substitution_ix env x t t' e e':
+      TYPE (insert env x t) e'             t' ->
+      TYPE env              e              t  ->
+      x <= length env                         ->
+      TYPE env              (subst e' e x) t'.
+Proof.
+ intros He' He Hlen.
+ remember (insert env x t) as ENV.
+ revert e x t env HeqENV He Hlen.
+ induction He'; intros; subst; simpl; try constructor; try assumption.
+  apply subst_cases; intros; subst.
+   eapply InEnv_insert in H. rewrite <- H. assumption.
+   apply insert_minus in H; try apply ty_env; try assumption; try omega.
+   apply insert_pre in H; try apply ty_env; try assumption; try omega.
+
+ eapply IHHe'; eauto; try reflexivity.
+  apply weakening_cons; assumption.
+  simpl; omega.
+
+ eapply ty_app.
+  eapply IHHe'1; auto.
+  eapply IHHe'2; auto.
+  assumption.
+
+ eapply IHHe'; simpl; try omega; try reflexivity.
+  apply weakening_cons.
+  assumption.
+
+ eapply IHHe'; eauto.
+ eapply IHHe'; eauto.
+Qed.
+
+
+Lemma substitution env t t' e e':
+      TYPE (t :: env)       e'             t' ->
+      TYPE env              e              t  ->
+      TYPE env              (subst e' e 0) t'.
+Proof.
+ intros.
+ eapply substitution_ix; try rewrite insert_0; try eassumption; try omega.
+Qed.
+
+
+Inductive val : Exp -> Prop :=
+ | v_lambda t b
+   : val (lambda t b)
+ | v_fold t e
+   : val e
+  -> val (fold t e)
+ | v_u
+   : val unitt.
+
+Inductive e_step: Exp -> Exp -> Prop :=
+ | e_ap1 e1 e1' e2
+   : e_step      e1          e1'
+  -> e_step (app e1 e2) (app e1' e2)
+ | e_ap2 e1 e2 e2'
+   : val e1
+  -> e_step         e2          e2'
+  -> e_step (app e1 e2) (app e1 e2')
+
+ | e_lam  t b x
+   : val x
+  -> e_step (app (lambda t b) x) (subst b x 0)
+
+ | e_fixx t e
+   : e_step (fixx t e) (subst e (fixx t e) 0)
+
+
+ | e_fold t e e'
+   : e_step e e'
+  -> e_step (fold t e) (fold t e')
+
+ | e_unfold1 e e'
+   : e_step e e'
+  -> e_step (unfold e) (unfold e')
+ | e_unfoldF t e
+   : val (fold t e)
+  -> e_step (unfold (fold t e)) e.
+
+
+
+Theorem preservation env e e' t:
+        TYPE env e t ->
+        e_step e e'  ->
+        TYPE env e' t.
+Proof.
+ intros Ht He.
+ revert env t Ht.
+ induction He; intros; inversion Ht; subst;
+   try solve [try econstructor; try eapply IHHe; eassumption];
+   try (eapply substitution; eassumption).
+  inversion H2. subst.
+  eapply substitution; eassumption.
+  inversion H1; subst; assumption.
+Qed.
+
+
+Theorem progress e t:
+        TYPE [] e t ->
+        val e \/ exists e', e_step e e'.
+Proof.
+ remember [] as ENV.
+ intros Ht.
+ induction Ht; subst;
+  try solve [apply not_InEnv_nil in H; destruct H];
+  try solve [left; econstructor; eassumption].
+
+ destruct IHHt1; try reflexivity.
+ destruct IHHt2; try reflexivity.
+ inversion H0; subst; inversion Ht1; subst.
+ right.
+  eexists. apply e_lam. assumption.
+ destruct H1.
+ right.
+  eexists. apply e_ap2; eassumption.
+ 
+ destruct H0.
+ right.
+  eexists. apply e_ap1; eassumption.
+
+ right. eexists. eapply e_fixx.
+
+ destruct IHHt; try reflexivity.
+  left. constructor. assumption.
+  destruct H0.
+   right. eexists. constructor. eassumption.
+
+ destruct IHHt; auto.
+  inversion H0; subst; inversion Ht; subst.
+  right. eexists. apply e_unfoldF. assumption.
+
+  destruct H0.
+  right. eexists. apply e_unfold1. eassumption.
+Qed.
